feat(pweak): define omega-frontier weak bisimulation

theories/Eq/PWeakUnbounded.v
@@ -1,7 +1,10 @@
 Set Warnings "-notation-overridden".
 Set Warnings "-ambiguous-paths".
 
-Require Import Utf8.
+Require Import Utf8 Program.
+
+From Coinduction Require Import all.
+From mathcomp Require Import eqtype.
 
 From PTree.Core Require Import PTreeDefinitionNew.
 From PTree.Prob Require Import FrontierLift MeasureIteration.
@@ -49,3 +52,97 @@ Lemma aufrontier_iter_unique
 Proof. eapply meas_iter_unique. Qed.
 
 End UnboundedFrontier.
+
+Section UnboundedWeak.
+Context {E : Type -> Type} {M : Type -> Type}
+  `{MI : MeasureInterface M}
+  `{MC : @MeasureCoreLaws M MI}
+  `{MO : @MeasureOmegaInterface M MI}.
+Context {R1 R2 : Type}.
+Variable RR : R1 -> R2 -> Prop.
+
+Definition aufrontier_match
+    (sim : ptree E M R1 -> ptree E M R2 -> Prop)
+    (ot1 : ptree' E M R1) (ot2 : ptree' E M R2) : Prop :=
+  (forall hs1, aufrontier ot1 hs1 -> exists hs2,
+      aufrontier ot2 hs2 /\ meas_lift (aphead_rel RR sim) hs1 hs2) /\
+  (forall hs2, aufrontier ot2 hs2 -> exists hs1,
+      aufrontier ot1 hs1 /\ meas_lift (aphead_rel RR sim) hs1 hs2).
+
+Inductive auweakF
+    (sim : ptree E M R1 -> ptree E M R2 -> Prop) :
+    ptree' E M R1 -> ptree' E M R2 -> Prop :=
+  | AUWFrontier ot1 ot2 hs1 hs2 :
+      aufrontier ot1 hs1 -> aufrontier ot2 hs2 ->
+      meas_lift (aphead_rel RR sim) hs1 hs2 ->
+      auweakF sim ot1 ot2
+  | AUWTau t1 t2 :
+      aufrontier_match sim (TauF t1) (TauF t2) ->
+      sim t1 t2 -> auweakF sim (TauF t1) (TauF t2)
+  | AUWProb {X Y : eqType} (mu : M X) (nu : M Y) k1 k2 :
+      aufrontier_match sim (ProbF mu k1) (ProbF nu k2) ->
+      meas_lift (fun x y => sim (k1 x) (k2 y)) mu nu ->
+      auweakF sim (ProbF mu k1) (ProbF nu k2)
+  | AUWTauL t1 ot2 :
+      auweakF sim (observe t1) ot2 -> auweakF sim (TauF t1) ot2
+  | AUWTauR ot1 t2 :
+      auweakF sim ot1 (observe t2) -> auweakF sim ot1 (TauF t2).
+
+Lemma auweakF_monotone sim1 sim2 :
+  (forall t1 t2, sim1 t1 t2 -> sim2 t1 t2) ->
+  forall ot1 ot2, auweakF sim1 ot1 ot2 -> auweakF sim2 ot1 ot2.
+Proof.
+  intros Hsim ot1 ot2 Hstep. induction Hstep.
+  - eapply AUWFrontier; [exact H|exact H0|].
+    eapply meas_lift_mono; [|exact H1].
+    eapply aphead_rel_mono. exact Hsim.
+  - apply AUWTau.
+    + destruct H as [HL HR]. split; intros hs Hf.
+      * destruct (HL hs Hf) as [hs' [Hf' Hlift]].
+        exists hs'. split; [exact Hf'|].
+        eapply meas_lift_mono; [|exact Hlift].
+        eapply aphead_rel_mono. exact Hsim.
+      * destruct (HR hs Hf) as [hs' [Hf' Hlift]].
+        exists hs'. split; [exact Hf'|].
+        eapply meas_lift_mono; [|exact Hlift].
+        eapply aphead_rel_mono. exact Hsim.
+    + exact (Hsim _ _ H0).
+  - apply AUWProb.
+    + destruct H as [HL HR]. split; intros hs Hf.
+      * destruct (HL hs Hf) as [hs' [Hf' Hlift]].
+        exists hs'. split; [exact Hf'|].
+        eapply meas_lift_mono; [|exact Hlift].
+        eapply aphead_rel_mono. exact Hsim.
+      * destruct (HR hs Hf) as [hs' [Hf' Hlift]].
+        exists hs'. split; [exact Hf'|].
+        eapply meas_lift_mono; [|exact Hlift].
+        eapply aphead_rel_mono. exact Hsim.
+    + eapply meas_lift_mono; [|exact H0].
+      intros x y Hxy. exact (Hsim _ _ Hxy).
+  - exact (AUWTauL IHHstep).
+  - exact (AUWTauR IHHstep).
+Qed.
+
+Definition auweak_body sim (t1 : ptree E M R1) (t2 : ptree E M R2) :=
+  auweakF sim (observe t1) (observe t2).
+
+Program Definition fauweak :
+    mon (ptree E M R1 -> ptree E M R2 -> Prop) :=
+  {| body := auweak_body |}.
+Next Obligation.
+  intros sim1 sim2 Hsub t1 t2 H.
+  eapply auweakF_monotone; eauto.
+Qed.
+
+Definition auweak : ptree E M R1 -> ptree E M R2 -> Prop :=
+  gfp fauweak.
+
+Lemma auweak_unfold t1 t2 :
+  auweak t1 t2 -> auweakF auweak (observe t1) (observe t2).
+Proof. intro H. apply (gfp_pfp fauweak) in H. exact H. Qed.
+
+Lemma auweak_fold t1 t2 :
+  auweakF auweak (observe t1) (observe t2) -> auweak t1 t2.
+Proof. intro H. unfold auweak. apply (gfp_fp fauweak). exact H. Qed.
+
+End UnboundedWeak.
